more boring lemmas

VCVio/OracleComp/SimSemantics/QueryTracking/CachingOracle.lean
@@ -11,47 +11,74 @@ import VCVio.OracleComp.Constructions.UniformSelect
 
 -/
 
-open Option
+open OracleComp OracleSpec
 
-variable {ι : Type} {spec : OracleSpec ι} {α β : Type}
+variable {ι : Type} [DecidableEq ι] {spec : OracleSpec ι} {α β : Type}
 
 namespace OracleSpec
 
-def QueryCache {ι : Type} (spec : OracleSpec ι) : Type :=
+/-- Type to represent a cache of queries to oracles in `spec`.
+Defined to be a function from (indexed) inputs to an optional output. -/
+def QueryCache (spec : OracleSpec ι) : Type :=
   (i : ι) → spec.domain i → Option (spec.range i)
 
-instance : EmptyCollection (QueryCache spec) := ⟨λ _ _ ↦ none⟩
+namespace QueryCache
 
-def QueryCache.cacheQuery {ι : Type} [DecidableEq ι] {spec : OracleSpec ι}
-    (cache : QueryCache spec) (i : ι)
-    (t : spec.domain i) (u : spec.range i) : QueryCache spec :=
-  Function.update cache i (Function.update (cache i) t u)
+variable (cache : QueryCache spec)
 
 instance : EmptyCollection (QueryCache spec) := ⟨λ _ _ ↦ none⟩
+
+section cacheQuery
+
+/-- Add a index + input pair to the cache by updating the function -/
+def cacheQuery (i : ι) (t : spec.domain i) (u : spec.range i) :
+    QueryCache spec := Function.update cache i (Function.update (cache i) t u)
+
+lemma cacheQuery_eq_ite_ite (i : ι) (t : spec.domain i) (u : spec.range i) :
+    cache.cacheQuery i t u = λ j t' ↦
+      if h : j = i then (if h ▸ t' = t then some (h ▸ u) else cache j t') else cache j t' := by
+  refine funext (λ j ↦ funext (λ t' ↦ ?_))
+  by_cases h : j = i
+  · induction h
+    by_cases ht : t' = t
+    · simp [ht, cacheQuery]
+    · simp [ht, cacheQuery]
+  · simp [h, cacheQuery]
+
+end cacheQuery
+
+section lookup_or_query
+
+variable {ι' : Type} {spec' : OracleSpec ι'}
+
+/-- Lookup a value in the cache, querying a fresh value if no value is cached.
+Returns both the value and updated cache. -/
+def lookup_or_else (cache : QueryCache spec) (i : ι) (t : spec.domain i)
+    (oq : OracleComp spec' (spec.range i)) :
+    OracleComp spec' (spec.range i × QueryCache spec) :=
+  match cache i t with
+  | Option.some u => return (u, cache)
+  | Option.none => do let u ← oq; return (u, cache.cacheQuery i t u)
+
+@[simp]
+lemma lookup_or_else_empty (i : ι) (t : spec.domain i) (oq : OracleComp spec' (spec.range i)) :
+    lookup_or_else ∅ i t oq = do let u ← oq; return (u, cacheQuery ∅ i t u) := rfl
+
+end lookup_or_query
+
+end QueryCache
 
 end OracleSpec
 
-open OracleComp OracleSpec
-
+/-- Oracle for caching queries to the oracles in `spec`, querying fresh values if needed. -/
 def cachingOracle {ι : Type} [DecidableEq ι] {spec : OracleSpec ι} :
     spec →[QueryCache spec]ₛₒ spec :=
-  λ i t cache ↦ match cache i t with
-    | Option.some u => return (u, cache)
-    | Option.none => do let u ← query i t; return (u, cache.cacheQuery i t u)
+  λ i t cache ↦ cache.lookup_or_else i t (query i t)
 
 namespace cachingOracle
 
--- port
+@[simp]
+lemma apply_eq (i : ι) (t : spec.domain i) (cache : QueryCache spec) :
+    cachingOracle i t cache = cache.lookup_or_else i t (query i t) := rfl
 
 end cachingOracle
-
-def randOracle {ι : Type} [DecidableEq ι] {spec : OracleSpec ι}
-    [∀ i, SelectableType (spec.range i)] :
-    spec →[QueryCache spec]ₛₒ unifSpec :=
-  (unifOracle ∘ₛₒ cachingOracle).maskState (Equiv.prodPUnit (QueryCache spec))
-
-namespace randOracle
-
--- port
-
-end randOracle
